src/Verification.v
@@ -90,19 +90,73 @@ Proof.
   induction i; dependent destruction p; destruct h; simpl;
   try (now reflexivity); try (apply IHi).
 Qed.
+(*should prove another lemma generalizing this one for N compiled instructions*)
+(*should find a lemma as general as this one for link*)
 
-(*should prove a lemma stating that linking doesn't affect non-jump instrs*)
-
-Lemma read_comp_ptrinc {n m} : forall p H1 H2, Language.read_instr p Language.PtrInc -> Assembly.read_instr (@Compiler.compile_link n m p H1 H2) (Assembly.Add 1).
+Lemma link_stable : forall n p ind i, (i <> Assembly.UJUMP /\ i <> Assembly.URET) ->
+                    p[@ind] = i -> (@Compiler.link n p)[@ind] = i.
 Admitted.
   
+Lemma read_comp_ptrinc {n m} : forall p H1 H2, Language.read_instr p Language.PtrInc -> Assembly.read_instr (@Compiler.compile_link n m p H1 H2) (Assembly.Add 1).
+Proof.
+  unfold Compiler.compile_link.
+  unfold Compiler.compile'.
+  intros.
+  ssimpl.
+  unfold Language.read_instr' in H0.
+  apply Assembly.ri.
+  unfold Assembly.read_instr'. simpl.
+  assert ((Compiler.compile'' prog)[@Compiler.compile_index prog pc] =
+  @Compiler.compile_first n prog[@pc]).
+  apply read_instr_eq.
+  rewrite H0 in H.
+  simpl in H.
+  apply link_stable.
+  split; discriminate.
+  assumption.
+Qed.
+  
+  
 Lemma read_comp_ptrdec {n m} : forall p H1 H2, Language.read_instr p Language.PtrDec -> Assembly.read_instr (@Compiler.compile_link n m p H1 H2) (Assembly.Sub 1).
-Admitted.
+Proof.
+  unfold Compiler.compile_link.
+  unfold Compiler.compile'.
+  intros.
+  ssimpl.
+  unfold Language.read_instr' in H0.
+  apply Assembly.ri.
+  unfold Assembly.read_instr'. simpl.
+  assert ((Compiler.compile'' prog)[@Compiler.compile_index prog pc] =
+  @Compiler.compile_first n prog[@pc]).
+  apply read_instr_eq.
+  rewrite H0 in H.
+  simpl in H.
+  apply link_stable.
+  split; discriminate.
+  assumption.
+Qed.
 
 Lemma read_comp_halt {n m} : forall p H1 H2, Language.read_instr p Language.Halt -> Assembly.read_instr (@Compiler.compile_link n m p H1 H2) (Assembly.Halt).
-Admitted.
+Proof.
+  unfold Compiler.compile_link.
+  unfold Compiler.compile'.
+  intros.
+  ssimpl.
+  unfold Language.read_instr' in H0.
+  apply Assembly.ri.
+  unfold Assembly.read_instr'. simpl.
+  assert ((Compiler.compile'' prog)[@Compiler.compile_index prog pc] =
+  @Compiler.compile_first n prog[@pc]).
+  apply read_instr_eq.
+  rewrite H0 in H.
+  simpl in H.
+  apply link_stable.
+  split; discriminate.
+  assumption.
+Qed.
 
-Lemma compiled_pc : forall n prog pc pc0 i, Language.read_instr' prog pc0 = i -> Language.to_nat pc0 + 1 = Language.to_nat pc -> Assembly.to_nat (Compiler.compile_index prog pc0) + vec_len (@Compiler.compile_one n i) = Assembly.to_nat (@Compiler.compile_index n prog pc).
+Lemma compiled_pc : forall n prog pc pc0 i, Language.read_instr' prog pc0 = i -> Common.to_nat pc0 + 1 = Common.to_nat pc -> Common.to_nat (Compiler.compile_index prog pc0) + vec_len (@Compiler.compile_one n i) = Common.to_nat (@Compiler.compile_index n prog pc).
+Proof.
 Admitted.
 
 Theorem comp_correct {n m : nat} :
@@ -134,6 +188,7 @@ Proof.
        apply read_comp_ptrinc. ssimpl.
        assumption.
       * simpl.
+        unfold Common.to_nat.
         apply compiled_pc with (i := Language.PtrInc); assumption.
       * now reflexivity.
       * now reflexivity.
